examples/listcopy.v
@@ -8,21 +8,31 @@ From SSL
 Require Import core.
 
 Inductive lseg (x : ptr) (s : seq nat) (h : heap) : Prop :=
-| lseg1 of x == null of
+| lseg_1 of x == null of
   @perm_eq nat_eqType (s) (nil) /\ h = empty
-| lseg2 of ~~ (x == null) of
+| lseg_2 of (x == null) = false of
   exists (v : nat) (s1 : seq nat) (nxt : ptr),
-  exists h_lseg_nxts1_515,
-  @perm_eq nat_eqType (s) ([:: v] ++ s1) /\ h = x :-> v \+ x .+ 1 :-> nxt \+ h_lseg_nxts1_515 /\ lseg nxt s1 h_lseg_nxts1_515.
+  exists h_lseg_nxts1_516,
+  @perm_eq nat_eqType (s) ([:: v] ++ s1) /\ h = x :-> v \+ x .+ 1 :-> nxt \+ h_lseg_nxts1_516 /\ lseg nxt s1 h_lseg_nxts1_516.
 
-Lemma lseg_perm_eq_trans5 x h s_1 s_2 : perm_eq s_1 s_2 -> lseg x s_1 h -> lseg x s_2 h. Admitted.
-Hint Resolve lseg_perm_eq_trans5: ssl_pred.
-Lemma pure6 : @perm_eq nat_eqType (nil) (nil). Admitted.
-Hint Resolve pure6: ssl_pure.
-Lemma pure7 vx22 s1x2 : @perm_eq nat_eqType ([:: vx22] ++ s1x2) ([:: vx22] ++ s1x2). Admitted.
-Hint Resolve pure7: ssl_pure.
-Lemma pure8 vx22 s1x2 : @perm_eq nat_eqType ([:: vx22] ++ s1x2) ([:: vx22] ++ s1x2). Admitted.
+Inductive lseg2 (x : ptr) (y : ptr) (s : seq nat) (h : heap) : Prop :=
+| lseg2_1 of x == y of
+  @perm_eq nat_eqType (s) (nil) /\ h = empty
+| lseg2_2 of (x == y) = false of
+  exists (v : nat) (s1 : seq nat) (nxt : ptr),
+  exists h_lseg2_nxtys1_517,
+  @perm_eq nat_eqType (s) ([:: v] ++ s1) /\ h = x :-> v \+ x .+ 1 :-> nxt \+ h_lseg2_nxtys1_517 /\ lseg2 nxt y s1 h_lseg2_nxtys1_517.
+
+Lemma lseg_perm_eq_trans6 x h s_1 s_2 : perm_eq s_1 s_2 -> lseg x s_1 h -> lseg x s_2 h. Admitted.
+Hint Resolve lseg_perm_eq_trans6: ssl_pred.
+Lemma lseg2_perm_eq_trans7 x y h s_1 s_2 : perm_eq s_1 s_2 -> lseg2 x y s_1 h -> lseg2 x y s_2 h. Admitted.
+Hint Resolve lseg2_perm_eq_trans7: ssl_pred.
+Lemma pure8 : @perm_eq nat_eqType (nil) (nil). Admitted.
 Hint Resolve pure8: ssl_pure.
+Lemma pure9 vx22 s1x2 : @perm_eq nat_eqType ([:: vx22] ++ s1x2) ([:: vx22] ++ s1x2). Admitted.
+Hint Resolve pure9: ssl_pure.
+Lemma pure10 vx22 s1x2 : @perm_eq nat_eqType ([:: vx22] ++ s1x2) ([:: vx22] ++ s1x2). Admitted.
+Hint Resolve pure10: ssl_pure.
 
 Definition listcopy_type :=
   forall (vprogs : ptr),
@@ -31,14 +41,14 @@ Definition listcopy_type :=
     fun h =>
       let: (r) := vprogs in
       let: (x, s) := vghosts in
-      exists h_lseg_xs_516,
-      h = r :-> x \+ h_lseg_xs_516 /\ lseg x s h_lseg_xs_516,
+      exists h_lseg_xs_518,
+      h = r :-> x \+ h_lseg_xs_518 /\ lseg x s h_lseg_xs_518,
     [vfun (_: unit) h =>
       let: (r) := vprogs in
       let: (x, s) := vghosts in
       exists y,
-      exists h_lseg_xs_517 h_lseg_ys_518,
-      h = r :-> y \+ h_lseg_xs_517 \+ h_lseg_ys_518 /\ lseg x s h_lseg_xs_517 /\ lseg y s h_lseg_ys_518
+      exists h_lseg_xs_519 h_lseg_ys_520,
+      h = r :-> y \+ h_lseg_xs_519 \+ h_lseg_ys_520 /\ lseg x s h_lseg_xs_519 /\ lseg y s h_lseg_ys_520
     ]).
 
 Program Definition listcopy : listcopy_type :=
@@ -65,16 +75,16 @@ Obligation Tactic := intro; move=>r; ssl_program_simpl.
 Next Obligation.
 ssl_ghostelim_pre.
 move=>[x2 s].
-ex_elim h_lseg_x2s_516.
+ex_elim h_lseg_x2s_518.
 move=>[sigma_self].
 subst.
-move=>H_lseg_x2s_516.
+move=>H_lseg_x2s_518.
 ssl_ghostelim_post.
 ssl_read r.
 ssl_open.
-ssl_open_post H_lseg_x2s_516.
-move=>[phi_lseg_x2s_5160].
-move=>[sigma_lseg_x2s_516].
+ssl_open_post H_lseg_x2s_518.
+move=>[phi_lseg_x2s_5180].
+move=>[sigma_lseg_x2s_518].
 subst.
 ssl_emp;
 exists (null);
@@ -85,26 +95,26 @@ unfold_constructor 1;
 sslauto.
 unfold_constructor 1;
 sslauto.
-ssl_open_post H_lseg_x2s_516.
+ssl_open_post H_lseg_x2s_518.
 ex_elim vx22 s1x2 nxtx22.
-ex_elim h_lseg_nxtx22s1x2_515x2.
-move=>[phi_lseg_x2s_5160].
-move=>[sigma_lseg_x2s_516].
+ex_elim h_lseg_nxtx22s1x2_516x2.
+move=>[phi_lseg_x2s_5180].
+move=>[sigma_lseg_x2s_518].
 subst.
-move=>H_lseg_nxtx22s1x2_515x2.
+move=>H_lseg_nxtx22s1x2_516x2.
 ssl_read x2.
 ssl_read (x2 .+ 1).
 ssl_write r.
-ssl_call_pre (r :-> nxtx22 \+ h_lseg_nxtx22s1x2_515x2).
+ssl_call_pre (r :-> nxtx22 \+ h_lseg_nxtx22s1x2_516x2).
 ssl_call (nxtx22, s1x2).
-exists (h_lseg_nxtx22s1x2_515x2);
+exists (h_lseg_nxtx22s1x2_516x2);
 sslauto.
 move=>h_call1.
 ex_elim y12.
-ex_elim h_lseg_nxtx22s1x2_5171 h_lseg_y12s1x2_5181.
+ex_elim h_lseg_nxtx22s1x2_5191 h_lseg_y12s1x2_5201.
 move=>[sigma_call1].
 subst.
-move=>[H_lseg_nxtx22s1x2_5171 H_lseg_y12s1x2_5181].
+move=>[H_lseg_nxtx22s1x2_5191 H_lseg_y12s1x2_5201].
 store_valid.
 ssl_read r.
 ssl_alloc y2.
@@ -116,15 +126,15 @@ ssl_write y2.
 ssl_write_post y2.
 ssl_emp;
 exists (y2);
-exists (x2 :-> vx22 \+ x2 .+ 1 :-> nxtx22 \+ h_lseg_nxtx22s1x2_5171);
-exists (y2 :-> vx22 \+ y2 .+ 1 :-> y12 \+ h_lseg_y12s1x2_5181);
+exists (x2 :-> vx22 \+ x2 .+ 1 :-> nxtx22 \+ h_lseg_nxtx22s1x2_5191);
+exists (y2 :-> vx22 \+ y2 .+ 1 :-> y12 \+ h_lseg_y12s1x2_5201);
 sslauto.
 unfold_constructor 2;
 exists (vx22), (s1x2), (nxtx22);
-exists (h_lseg_nxtx22s1x2_5171);
+exists (h_lseg_nxtx22s1x2_5191);
 sslauto.
 unfold_constructor 2;
 exists (vx22), (s1x2), (y12);
-exists (h_lseg_y12s1x2_5181);
+exists (h_lseg_y12s1x2_5201);
 sslauto.
 Qed.
