examples/listfree.v
@@ -8,15 +8,25 @@ From SSL
 Require Import core.
 
 Inductive lseg (x : ptr) (s : seq nat) (h : heap) : Prop :=
-| lseg1 of x == null of
+| lseg_1 of x == null of
   @perm_eq nat_eqType (s) (nil) /\ h = empty
-| lseg2 of ~~ (x == null) of
+| lseg_2 of (x == null) = false of
   exists (v : nat) (s1 : seq nat) (nxt : ptr),
   exists h_lseg_nxts1_513,
   @perm_eq nat_eqType (s) ([:: v] ++ s1) /\ h = x :-> v \+ x .+ 1 :-> nxt \+ h_lseg_nxts1_513 /\ lseg nxt s1 h_lseg_nxts1_513.
 
+Inductive lseg2 (x : ptr) (y : ptr) (s : seq nat) (h : heap) : Prop :=
+| lseg2_1 of x == y of
+  @perm_eq nat_eqType (s) (nil) /\ h = empty
+| lseg2_2 of (x == y) = false of
+  exists (v : nat) (s1 : seq nat) (nxt : ptr),
+  exists h_lseg2_nxtys1_514,
+  @perm_eq nat_eqType (s) ([:: v] ++ s1) /\ h = x :-> v \+ x .+ 1 :-> nxt \+ h_lseg2_nxtys1_514 /\ lseg2 nxt y s1 h_lseg2_nxtys1_514.
+
 Lemma lseg_perm_eq_trans4 x h s_1 s_2 : perm_eq s_1 s_2 -> lseg x s_1 h -> lseg x s_2 h. Admitted.
 Hint Resolve lseg_perm_eq_trans4: ssl_pred.
+Lemma lseg2_perm_eq_trans5 x y h s_1 s_2 : perm_eq s_1 s_2 -> lseg2 x y s_1 h -> lseg2 x y s_2 h. Admitted.
+Hint Resolve lseg2_perm_eq_trans5: ssl_pred.
 
 Definition listfree_type :=
   forall (vprogs : ptr),
@@ -25,8 +35,8 @@ Definition listfree_type :=
     fun h =>
       let: (x) := vprogs in
       let: (s) := vghosts in
-      exists h_lseg_xs_514,
-      h = h_lseg_xs_514 /\ lseg x s h_lseg_xs_514,
+      exists h_lseg_xs_515,
+      h = h_lseg_xs_515 /\ lseg x s h_lseg_xs_515,
     [vfun (_: unit) h =>
       let: (x) := vprogs in
       let: (s) := vghosts in
@@ -51,23 +61,23 @@ Obligation Tactic := intro; move=>x; ssl_program_simpl.
 Next Obligation.
 ssl_ghostelim_pre.
 move=>s.
-ex_elim h_lseg_xs_514.
+ex_elim h_lseg_xs_515.
 move=>[sigma_self].
 subst.
-move=>H_lseg_xs_514.
+move=>H_lseg_xs_515.
 ssl_ghostelim_post.
 ssl_open.
-ssl_open_post H_lseg_xs_514.
-move=>[phi_lseg_xs_5140].
-move=>[sigma_lseg_xs_514].
+ssl_open_post H_lseg_xs_515.
+move=>[phi_lseg_xs_5150].
+move=>[sigma_lseg_xs_515].
 subst.
 ssl_emp;
 sslauto.
-ssl_open_post H_lseg_xs_514.
+ssl_open_post H_lseg_xs_515.
 ex_elim vx2 s1x nxtx2.
 ex_elim h_lseg_nxtx2s1x_513x.
-move=>[phi_lseg_xs_5140].
-move=>[sigma_lseg_xs_514].
+move=>[phi_lseg_xs_5150].
+move=>[sigma_lseg_xs_515].
 subst.
 move=>H_lseg_nxtx2s1x_513x.
 ssl_read (x .+ 1).
