examples/sll_append.v
@@ -8,17 +8,17 @@ From SSL
 Require Import core.
 
 Inductive sll (x : ptr) (s : seq nat) (h : heap) : Prop :=
-| sll1 of x == null of
+| sll_1 of x == null of
   @perm_eq nat_eqType (s) (nil) /\ h = empty
-| sll2 of ~~ (x == null) of
+| sll_2 of (x == null) = false of
   exists (v : nat) (s1 : seq nat) (nxt : ptr),
-  exists h_sll_nxts1_537,
-  @perm_eq nat_eqType (s) ([:: v] ++ s1) /\ h = x :-> v \+ x .+ 1 :-> nxt \+ h_sll_nxts1_537 /\ sll nxt s1 h_sll_nxts1_537.
+  exists h_sll_nxts1_543,
+  @perm_eq nat_eqType (s) ([:: v] ++ s1) /\ h = x :-> v \+ x .+ 1 :-> nxt \+ h_sll_nxts1_543 /\ sll nxt s1 h_sll_nxts1_543.
 
-Lemma sll_perm_eq_trans25 x h s_1 s_2 : perm_eq s_1 s_2 -> sll x s_1 h -> sll x s_2 h. Admitted.
-Hint Resolve sll_perm_eq_trans25: ssl_pred.
-Lemma pure26 vx12 s1x1 s2 : @perm_eq nat_eqType ([:: vx12] ++ s1x1 ++ s2) ([:: vx12] ++ s1x1 ++ s2). Admitted.
-Hint Resolve pure26: ssl_pure.
+Lemma sll_perm_eq_trans32 x h s_1 s_2 : perm_eq s_1 s_2 -> sll x s_1 h -> sll x s_2 h. Admitted.
+Hint Resolve sll_perm_eq_trans32: ssl_pred.
+Lemma pure33 vx12 s1x1 s2 : @perm_eq nat_eqType ([:: vx12] ++ s1x1 ++ s2) ([:: vx12] ++ s1x1 ++ s2). Admitted.
+Hint Resolve pure33: ssl_pure.
 
 Definition sll_append_type :=
   forall (vprogs : ptr * ptr),
@@ -27,14 +27,14 @@ Definition sll_append_type :=
     fun h =>
       let: (x1, r) := vprogs in
       let: (s1, x2, s2) := vghosts in
-      exists h_sll_x1s1_538 h_sll_x2s2_539,
-      h = r :-> x2 \+ h_sll_x1s1_538 \+ h_sll_x2s2_539 /\ sll x1 s1 h_sll_x1s1_538 /\ sll x2 s2 h_sll_x2s2_539,
+      exists h_sll_x1s1_544 h_sll_x2s2_545,
+      h = r :-> x2 \+ h_sll_x1s1_544 \+ h_sll_x2s2_545 /\ sll x1 s1 h_sll_x1s1_544 /\ sll x2 s2 h_sll_x2s2_545,
     [vfun (_: unit) h =>
       let: (x1, r) := vprogs in
       let: (s1, x2, s2) := vghosts in
       exists s y,
-      exists h_sll_ys_540,
-      @perm_eq nat_eqType (s) (s1 ++ s2) /\ h = r :-> y \+ h_sll_ys_540 /\ sll y s h_sll_ys_540
+      exists h_sll_ys_546,
+      @perm_eq nat_eqType (s) (s1 ++ s2) /\ h = r :-> y \+ h_sll_ys_546 /\ sll y s h_sll_ys_546
     ]).
 
 Program Definition sll_append : sll_append_type :=
@@ -56,40 +56,40 @@ Obligation Tactic := intro; move=>[x1 r]; ssl_program_simpl.
 Next Obligation.
 ssl_ghostelim_pre.
 move=>[[s1 x22] s2].
-ex_elim h_sll_x1s1_538 h_sll_x22s2_539.
+ex_elim h_sll_x1s1_544 h_sll_x22s2_545.
 move=>[sigma_self].
 subst.
-move=>[H_sll_x1s1_538 H_sll_x22s2_539].
+move=>[H_sll_x1s1_544 H_sll_x22s2_545].
 ssl_ghostelim_post.
 ssl_open.
-ssl_open_post H_sll_x1s1_538.
-move=>[phi_sll_x1s1_5380].
-move=>[sigma_sll_x1s1_538].
+ssl_open_post H_sll_x1s1_544.
+move=>[phi_sll_x1s1_5440].
+move=>[sigma_sll_x1s1_544].
 subst.
 ssl_emp;
 exists (nil ++ s2), (x22);
-exists (h_sll_x22s2_539);
+exists (h_sll_x22s2_545);
 sslauto.
-ssl_open_post H_sll_x1s1_538.
+ssl_open_post H_sll_x1s1_544.
 ex_elim vx12 s1x1 nxtx12.
-ex_elim h_sll_nxtx12s1x1_537x1.
-move=>[phi_sll_x1s1_5380].
-move=>[sigma_sll_x1s1_538].
+ex_elim h_sll_nxtx12s1x1_543x1.
+move=>[phi_sll_x1s1_5440].
+move=>[sigma_sll_x1s1_544].
 subst.
-move=>H_sll_nxtx12s1x1_537x1.
+move=>H_sll_nxtx12s1x1_543x1.
 ssl_read (x1 .+ 1).
-ssl_call_pre (r :-> x22 \+ h_sll_nxtx12s1x1_537x1 \+ h_sll_x22s2_539).
+ssl_call_pre (r :-> x22 \+ h_sll_nxtx12s1x1_543x1 \+ h_sll_x22s2_545).
 ssl_call (s1x1, x22, s2).
-exists (h_sll_nxtx12s1x1_537x1);
-exists (h_sll_x22s2_539);
+exists (h_sll_nxtx12s1x1_543x1);
+exists (h_sll_x22s2_545);
 sslauto.
 move=>h_call1.
 ex_elim s3 y12.
-ex_elim h_sll_y12s1x1s2_5401.
+ex_elim h_sll_y12s1x1s2_5461.
 move=>[phi_call10].
 move=>[sigma_call1].
 subst.
-move=>H_sll_y12s3_5401.
+move=>H_sll_y12s3_5461.
 store_valid.
 ssl_read r.
 ssl_write (x1 .+ 1).
@@ -98,10 +98,10 @@ ssl_write r.
 ssl_write_post r.
 ssl_emp;
 exists ([:: vx12] ++ s1x1 ++ s2), (x1);
-exists (x1 :-> vx12 \+ x1 .+ 1 :-> y12 \+ h_sll_y12s1x1s2_5401);
+exists (x1 :-> vx12 \+ x1 .+ 1 :-> y12 \+ h_sll_y12s1x1s2_5461);
 sslauto.
 unfold_constructor 2;
 exists (vx12), (s1x1 ++ s2), (y12);
-exists (h_sll_y12s1x1s2_5401);
+exists (h_sll_y12s1x1s2_5461);
 sslauto.
 Qed.
