examples/sll_copy.v
@@ -8,23 +8,23 @@ From SSL
 Require Import core.
 
 Inductive sll (x : ptr) (s : seq nat) (h : heap) : Prop :=
-| sll1 of x == null of
+| sll_1 of x == null of
   @perm_eq nat_eqType (s) (nil) /\ h = empty
-| sll2 of ~~ (x == null) of
+| sll_2 of (x == null) = false of
   exists (v : nat) (s1 : seq nat) (nxt : ptr),
-  exists h_sll_nxts1_534,
-  @perm_eq nat_eqType (s) ([:: v] ++ s1) /\ h = x :-> v \+ x .+ 1 :-> nxt \+ h_sll_nxts1_534 /\ sll nxt s1 h_sll_nxts1_534.
+  exists h_sll_nxts1_540,
+  @perm_eq nat_eqType (s) ([:: v] ++ s1) /\ h = x :-> v \+ x .+ 1 :-> nxt \+ h_sll_nxts1_540 /\ sll nxt s1 h_sll_nxts1_540.
 
-Lemma sll_perm_eq_trans19 x h s_1 s_2 : perm_eq s_1 s_2 -> sll x s_1 h -> sll x s_2 h. Admitted.
-Hint Resolve sll_perm_eq_trans19: ssl_pred.
-Lemma pure20 : @perm_eq nat_eqType (nil) (nil). Admitted.
-Hint Resolve pure20: ssl_pure.
-Lemma pure21 b1 : b1 < b1 + 1. Admitted.
-Hint Resolve pure21: ssl_pure.
-Lemma pure22 vx22 s1x2 : @perm_eq nat_eqType ([:: vx22] ++ s1x2) ([:: vx22] ++ s1x2). Admitted.
-Hint Resolve pure22: ssl_pure.
-Lemma pure23 vx22 s1x2 : @perm_eq nat_eqType ([:: vx22] ++ s1x2) ([:: vx22] ++ s1x2). Admitted.
-Hint Resolve pure23: ssl_pure.
+Lemma sll_perm_eq_trans26 x h s_1 s_2 : perm_eq s_1 s_2 -> sll x s_1 h -> sll x s_2 h. Admitted.
+Hint Resolve sll_perm_eq_trans26: ssl_pred.
+Lemma pure27 : @perm_eq nat_eqType (nil) (nil). Admitted.
+Hint Resolve pure27: ssl_pure.
+Lemma pure28 b1 : b1 < b1 + 1. Admitted.
+Hint Resolve pure28: ssl_pure.
+Lemma pure29 vx22 s1x2 : @perm_eq nat_eqType ([:: vx22] ++ s1x2) ([:: vx22] ++ s1x2). Admitted.
+Hint Resolve pure29: ssl_pure.
+Lemma pure30 vx22 s1x2 : @perm_eq nat_eqType ([:: vx22] ++ s1x2) ([:: vx22] ++ s1x2). Admitted.
+Hint Resolve pure30: ssl_pure.
 
 Definition sll_copy_type :=
   forall (vprogs : ptr),
@@ -89,24 +89,24 @@ unfold_constructor 1;
 sslauto.
 ssl_open_post H_sll_x2s_a.
 ex_elim vx22 s1x2 nxtx22.
-ex_elim h_sll_nxtx22s1x2_534x2.
+ex_elim h_sll_nxtx22s1x2_540x2.
 move=>[phi_sll_x2s_a0].
 move=>[sigma_sll_x2s_a].
 subst.
-move=>H_sll_nxtx22s1x2_534x2.
+move=>H_sll_nxtx22s1x2_540x2.
 ssl_read x2.
 ssl_read (x2 .+ 1).
 ssl_write r.
-ssl_call_pre (r :-> nxtx22 \+ h_sll_nxtx22s1x2_534x2).
+ssl_call_pre (r :-> nxtx22 \+ h_sll_nxtx22s1x2_540x2).
 ssl_call (nxtx22, s1x2).
-exists (h_sll_nxtx22s1x2_534x2);
+exists (h_sll_nxtx22s1x2_540x2);
 sslauto.
 move=>h_call1.
 ex_elim y12.
-ex_elim h_sll_nxtx22s1x2_534x2 h_sll_y12s1x2_b1.
+ex_elim h_sll_nxtx22s1x2_540x2 h_sll_y12s1x2_b1.
 move=>[sigma_call1].
 subst.
-move=>[H_sll_nxtx22s1x2_534x2 H_sll_y12s1x2_b1].
+move=>[H_sll_nxtx22s1x2_540x2 H_sll_y12s1x2_b1].
 store_valid.
 ssl_read r.
 ssl_alloc y2.
@@ -118,12 +118,12 @@ ssl_write y2.
 ssl_write_post y2.
 ssl_emp;
 exists (y2);
-exists (x2 :-> vx22 \+ x2 .+ 1 :-> nxtx22 \+ h_sll_nxtx22s1x2_534x2);
+exists (x2 :-> vx22 \+ x2 .+ 1 :-> nxtx22 \+ h_sll_nxtx22s1x2_540x2);
 exists (y2 :-> vx22 \+ y2 .+ 1 :-> y12 \+ h_sll_y12s1x2_b1);
 sslauto.
 unfold_constructor 2;
 exists (vx22), (s1x2), (nxtx22);
-exists (h_sll_nxtx22s1x2_534x2);
+exists (h_sll_nxtx22s1x2_540x2);
 sslauto.
 unfold_constructor 2;
 exists (vx22), (s1x2), (y12);
