examples/sll_free.v
@@ -8,15 +8,15 @@ From SSL
 Require Import core.
 
 Inductive sll (x : ptr) (s : seq nat) (h : heap) : Prop :=
-| sll1 of x == null of
+| sll_1 of x == null of
   @perm_eq nat_eqType (s) (nil) /\ h = empty
-| sll2 of ~~ (x == null) of
+| sll_2 of (x == null) = false of
   exists (v : nat) (s1 : seq nat) (nxt : ptr),
-  exists h_sll_nxts1_535,
-  @perm_eq nat_eqType (s) ([:: v] ++ s1) /\ h = x :-> v \+ x .+ 1 :-> nxt \+ h_sll_nxts1_535 /\ sll nxt s1 h_sll_nxts1_535.
+  exists h_sll_nxts1_541,
+  @perm_eq nat_eqType (s) ([:: v] ++ s1) /\ h = x :-> v \+ x .+ 1 :-> nxt \+ h_sll_nxts1_541 /\ sll nxt s1 h_sll_nxts1_541.
 
-Lemma sll_perm_eq_trans24 x h s_1 s_2 : perm_eq s_1 s_2 -> sll x s_1 h -> sll x s_2 h. Admitted.
-Hint Resolve sll_perm_eq_trans24: ssl_pred.
+Lemma sll_perm_eq_trans31 x h s_1 s_2 : perm_eq s_1 s_2 -> sll x s_1 h -> sll x s_2 h. Admitted.
+Hint Resolve sll_perm_eq_trans31: ssl_pred.
 
 Definition sll_free_type :=
   forall (vprogs : ptr),
@@ -25,8 +25,8 @@ Definition sll_free_type :=
     fun h =>
       let: (x) := vprogs in
       let: (s) := vghosts in
-      exists h_sll_xs_536,
-      h = h_sll_xs_536 /\ sll x s h_sll_xs_536,
+      exists h_sll_xs_542,
+      h = h_sll_xs_542 /\ sll x s h_sll_xs_542,
     [vfun (_: unit) h =>
       let: (x) := vprogs in
       let: (s) := vghosts in
@@ -51,29 +51,29 @@ Obligation Tactic := intro; move=>x; ssl_program_simpl.
 Next Obligation.
 ssl_ghostelim_pre.
 move=>s.
-ex_elim h_sll_xs_536.
+ex_elim h_sll_xs_542.
 move=>[sigma_self].
 subst.
-move=>H_sll_xs_536.
+move=>H_sll_xs_542.
 ssl_ghostelim_post.
 ssl_open.
-ssl_open_post H_sll_xs_536.
-move=>[phi_sll_xs_5360].
-move=>[sigma_sll_xs_536].
+ssl_open_post H_sll_xs_542.
+move=>[phi_sll_xs_5420].
+move=>[sigma_sll_xs_542].
 subst.
 ssl_emp;
 sslauto.
-ssl_open_post H_sll_xs_536.
+ssl_open_post H_sll_xs_542.
 ex_elim vx2 s1x nxtx2.
-ex_elim h_sll_nxtx2s1x_535x.
-move=>[phi_sll_xs_5360].
-move=>[sigma_sll_xs_536].
+ex_elim h_sll_nxtx2s1x_541x.
+move=>[phi_sll_xs_5420].
+move=>[sigma_sll_xs_542].
 subst.
-move=>H_sll_nxtx2s1x_535x.
+move=>H_sll_nxtx2s1x_541x.
 ssl_read (x .+ 1).
-ssl_call_pre (h_sll_nxtx2s1x_535x).
+ssl_call_pre (h_sll_nxtx2s1x_541x).
 ssl_call (s1x).
-exists (h_sll_nxtx2s1x_535x);
+exists (h_sll_nxtx2s1x_541x);
 sslauto.
 move=>h_call1.
 move=>[sigma_call1].
