examples/sll_init.v
@@ -8,19 +8,19 @@ From SSL
 Require Import core.
 
 Inductive sll (x : ptr) (s : seq nat) (h : heap) : Prop :=
-| sll1 of x == null of
+| sll_1 of x == null of
   @perm_eq nat_eqType (s) (nil) /\ h = empty
-| sll2 of ~~ (x == null) of
+| sll_2 of (x == null) = false of
   exists (v : nat) (s1 : seq nat) (nxt : ptr),
-  exists h_sll_nxts1_543,
-  @perm_eq nat_eqType (s) ([:: v] ++ s1) /\ h = x :-> v \+ x .+ 1 :-> nxt \+ h_sll_nxts1_543 /\ sll nxt s1 h_sll_nxts1_543.
+  exists h_sll_nxts1_549,
+  @perm_eq nat_eqType (s) ([:: v] ++ s1) /\ h = x :-> v \+ x .+ 1 :-> nxt \+ h_sll_nxts1_549 /\ sll nxt s1 h_sll_nxts1_549.
 
-Lemma sll_perm_eq_trans29 x h s_1 s_2 : perm_eq s_1 s_2 -> sll x s_1 h -> sll x s_2 h. Admitted.
-Hint Resolve sll_perm_eq_trans29: ssl_pred.
-Lemma pure30 v : @sub_mem nat_eqType (mem (nil)) (mem ([:: v])). Admitted.
-Hint Resolve pure30: ssl_pure.
-Lemma pure31 v s11 : @sub_mem nat_eqType (mem (s11)) (mem ([:: v])) -> @sub_mem nat_eqType (mem ([:: v] ++ s11)) (mem ([:: v])). Admitted.
-Hint Resolve pure31: ssl_pure.
+Lemma sll_perm_eq_trans36 x h s_1 s_2 : perm_eq s_1 s_2 -> sll x s_1 h -> sll x s_2 h. Admitted.
+Hint Resolve sll_perm_eq_trans36: ssl_pred.
+Lemma pure37 v : @sub_mem nat_eqType (mem (nil)) (mem ([:: v])). Admitted.
+Hint Resolve pure37: ssl_pure.
+Lemma pure38 v s11 : @sub_mem nat_eqType (mem (s11)) (mem ([:: v])) -> @sub_mem nat_eqType (mem ([:: v] ++ s11)) (mem ([:: v])). Admitted.
+Hint Resolve pure38: ssl_pure.
 
 Definition sll_init_type :=
   forall (vprogs : ptr * nat),
@@ -29,14 +29,14 @@ Definition sll_init_type :=
     fun h =>
       let: (x, v) := vprogs in
       let: (s) := vghosts in
-      exists h_sll_xs_544,
-      h = h_sll_xs_544 /\ sll x s h_sll_xs_544,
+      exists h_sll_xs_550,
+      h = h_sll_xs_550 /\ sll x s h_sll_xs_550,
     [vfun (_: unit) h =>
       let: (x, v) := vprogs in
       let: (s) := vghosts in
       exists s1,
-      exists h_sll_xs1_545,
-      @sub_mem nat_eqType (mem (s1)) (mem ([:: v])) /\ h = h_sll_xs1_545 /\ sll x s1 h_sll_xs1_545
+      exists h_sll_xs1_551,
+      @sub_mem nat_eqType (mem (s1)) (mem ([:: v])) /\ h = h_sll_xs1_551 /\ sll x s1 h_sll_xs1_551
     ]).
 
 Program Definition sll_init : sll_init_type :=
@@ -56,15 +56,15 @@ Obligation Tactic := intro; move=>[x v]; ssl_program_simpl.
 Next Obligation.
 ssl_ghostelim_pre.
 move=>s.
-ex_elim h_sll_xs_544.
+ex_elim h_sll_xs_550.
 move=>[sigma_self].
 subst.
-move=>H_sll_xs_544.
+move=>H_sll_xs_550.
 ssl_ghostelim_post.
 ssl_open.
-ssl_open_post H_sll_xs_544.
-move=>[phi_sll_xs_5440].
-move=>[sigma_sll_xs_544].
+ssl_open_post H_sll_xs_550.
+move=>[phi_sll_xs_5500].
+move=>[sigma_sll_xs_550].
 subst.
 ssl_emp;
 exists (nil);
@@ -72,34 +72,34 @@ exists (empty);
 sslauto.
 unfold_constructor 1;
 sslauto.
-ssl_open_post H_sll_xs_544.
+ssl_open_post H_sll_xs_550.
 ex_elim vx2 s1x nxtx2.
-ex_elim h_sll_nxtx2s1x_543x.
-move=>[phi_sll_xs_5440].
-move=>[sigma_sll_xs_544].
+ex_elim h_sll_nxtx2s1x_549x.
+move=>[phi_sll_xs_5500].
+move=>[sigma_sll_xs_550].
 subst.
-move=>H_sll_nxtx2s1x_543x.
+move=>H_sll_nxtx2s1x_549x.
 ssl_read (x .+ 1).
-ssl_call_pre (h_sll_nxtx2s1x_543x).
+ssl_call_pre (h_sll_nxtx2s1x_549x).
 ssl_call (s1x).
-exists (h_sll_nxtx2s1x_543x);
+exists (h_sll_nxtx2s1x_549x);
 sslauto.
 move=>h_call1.
 ex_elim s11.
-ex_elim h_sll_nxtx2s11_5451.
+ex_elim h_sll_nxtx2s11_5511.
 move=>[phi_call10].
 move=>[sigma_call1].
 subst.
-move=>H_sll_nxtx2s11_5451.
+move=>H_sll_nxtx2s11_5511.
 store_valid.
 ssl_write x.
 ssl_write_post x.
 ssl_emp;
 exists ([:: v] ++ s11);
-exists (x :-> v \+ x .+ 1 :-> nxtx2 \+ h_sll_nxtx2s11_5451);
+exists (x :-> v \+ x .+ 1 :-> nxtx2 \+ h_sll_nxtx2s11_5511);
 sslauto.
 unfold_constructor 2;
 exists (v), (s11), (nxtx2);
-exists (h_sll_nxtx2s11_5451);
+exists (h_sll_nxtx2s11_5511);
 sslauto.
 Qed.
