examples/sll_to_dll.v
@@ -8,31 +8,31 @@ From SSL
 Require Import core.
 
 Inductive dll (x : ptr) (z : ptr) (s : seq nat) (h : heap) : Prop :=
-| dll1 of x == null of
+| dll_1 of x == null of
   @perm_eq nat_eqType (s) (nil) /\ h = empty
-| dll2 of ~~ (x == null) of
+| dll_2 of (x == null) = false of
   exists (v : nat) (s1 : seq nat) (w : ptr),
-  exists h_dll_wxs1_552,
-  @perm_eq nat_eqType (s) ([:: v] ++ s1) /\ h = x :-> v \+ x .+ 1 :-> w \+ x .+ 2 :-> z \+ h_dll_wxs1_552 /\ dll w x s1 h_dll_wxs1_552.
+  exists h_dll_wxs1_558,
+  @perm_eq nat_eqType (s) ([:: v] ++ s1) /\ h = x :-> v \+ x .+ 1 :-> w \+ x .+ 2 :-> z \+ h_dll_wxs1_558 /\ dll w x s1 h_dll_wxs1_558.
 
 Inductive sll (x : ptr) (s : seq nat) (h : heap) : Prop :=
-| sll1 of x == null of
+| sll_1 of x == null of
   @perm_eq nat_eqType (s) (nil) /\ h = empty
-| sll2 of ~~ (x == null) of
+| sll_2 of (x == null) = false of
   exists (v : nat) (s1 : seq nat) (nxt : ptr),
-  exists h_sll_nxts1_553,
-  @perm_eq nat_eqType (s) ([:: v] ++ s1) /\ h = x :-> v \+ x .+ 1 :-> nxt \+ h_sll_nxts1_553 /\ sll nxt s1 h_sll_nxts1_553.
+  exists h_sll_nxts1_559,
+  @perm_eq nat_eqType (s) ([:: v] ++ s1) /\ h = x :-> v \+ x .+ 1 :-> nxt \+ h_sll_nxts1_559 /\ sll nxt s1 h_sll_nxts1_559.
 
-Lemma dll_perm_eq_trans38 x z h s_1 s_2 : perm_eq s_1 s_2 -> dll x z s_1 h -> dll x z s_2 h. Admitted.
-Hint Resolve dll_perm_eq_trans38: ssl_pred.
-Lemma sll_perm_eq_trans39 x h s_1 s_2 : perm_eq s_1 s_2 -> sll x s_1 h -> sll x s_2 h. Admitted.
-Hint Resolve sll_perm_eq_trans39: ssl_pred.
-Lemma pure40 : @perm_eq nat_eqType (nil) (nil). Admitted.
-Hint Resolve pure40: ssl_pure.
-Lemma pure41 vx22 : @perm_eq nat_eqType ([:: vx22]) ([:: vx22]). Admitted.
-Hint Resolve pure41: ssl_pure.
-Lemma pure42 vx22 vi122 s1i12 : @perm_eq nat_eqType ([:: vx22] ++ [:: vi122] ++ s1i12) ([:: vx22] ++ [:: vi122] ++ s1i12). Admitted.
-Hint Resolve pure42: ssl_pure.
+Lemma dll_perm_eq_trans45 x z h s_1 s_2 : perm_eq s_1 s_2 -> dll x z s_1 h -> dll x z s_2 h. Admitted.
+Hint Resolve dll_perm_eq_trans45: ssl_pred.
+Lemma sll_perm_eq_trans46 x h s_1 s_2 : perm_eq s_1 s_2 -> sll x s_1 h -> sll x s_2 h. Admitted.
+Hint Resolve sll_perm_eq_trans46: ssl_pred.
+Lemma pure47 : @perm_eq nat_eqType (nil) (nil). Admitted.
+Hint Resolve pure47: ssl_pure.
+Lemma pure48 vx22 : @perm_eq nat_eqType ([:: vx22]) ([:: vx22]). Admitted.
+Hint Resolve pure48: ssl_pure.
+Lemma pure49 vx22 vi122 s1i12 : @perm_eq nat_eqType ([:: vx22] ++ [:: vi122] ++ s1i12) ([:: vx22] ++ [:: vi122] ++ s1i12). Admitted.
+Hint Resolve pure49: ssl_pure.
 
 Definition sll_to_dll_type :=
   forall (vprogs : ptr),
@@ -41,14 +41,14 @@ Definition sll_to_dll_type :=
     fun h =>
       let: (f) := vprogs in
       let: (x, s) := vghosts in
-      exists h_sll_xs_554,
-      h = f :-> x \+ h_sll_xs_554 /\ sll x s h_sll_xs_554,
+      exists h_sll_xs_560,
+      h = f :-> x \+ h_sll_xs_560 /\ sll x s h_sll_xs_560,
     [vfun (_: unit) h =>
       let: (f) := vprogs in
       let: (x, s) := vghosts in
       exists i,
-      exists h_dll_is_555,
-      h = f :-> i \+ h_dll_is_555 /\ dll i null s h_dll_is_555
+      exists h_dll_is_561,
+      h = f :-> i \+ h_dll_is_561 /\ dll i null s h_dll_is_561
     ]).
 
 Program Definition sll_to_dll : sll_to_dll_type :=
@@ -90,16 +90,16 @@ Obligation Tactic := intro; move=>f; ssl_program_simpl.
 Next Obligation.
 ssl_ghostelim_pre.
 move=>[x2 s].
-ex_elim h_sll_x2s_554.
+ex_elim h_sll_x2s_560.
 move=>[sigma_self].
 subst.
-move=>H_sll_x2s_554.
+move=>H_sll_x2s_560.
 ssl_ghostelim_post.
 ssl_read f.
 ssl_open.
-ssl_open_post H_sll_x2s_554.
-move=>[phi_sll_x2s_5540].
-move=>[sigma_sll_x2s_554].
+ssl_open_post H_sll_x2s_560.
+move=>[phi_sll_x2s_5600].
+move=>[sigma_sll_x2s_560].
 subst.
 ssl_emp;
 exists (null);
@@ -107,32 +107,32 @@ exists (empty);
 sslauto.
 unfold_constructor 1;
 sslauto.
-ssl_open_post H_sll_x2s_554.
+ssl_open_post H_sll_x2s_560.
 ex_elim vx22 s1x2 nxtx22.
-ex_elim h_sll_nxtx22s1x2_553x2.
-move=>[phi_sll_x2s_5540].
-move=>[sigma_sll_x2s_554].
+ex_elim h_sll_nxtx22s1x2_559x2.
+move=>[phi_sll_x2s_5600].
+move=>[sigma_sll_x2s_560].
 subst.
-move=>H_sll_nxtx22s1x2_553x2.
+move=>H_sll_nxtx22s1x2_559x2.
 ssl_read x2.
 ssl_read (x2 .+ 1).
 ssl_write f.
-ssl_call_pre (f :-> nxtx22 \+ h_sll_nxtx22s1x2_553x2).
+ssl_call_pre (f :-> nxtx22 \+ h_sll_nxtx22s1x2_559x2).
 ssl_call (nxtx22, s1x2).
-exists (h_sll_nxtx22s1x2_553x2);
+exists (h_sll_nxtx22s1x2_559x2);
 sslauto.
 move=>h_call1.
 ex_elim i12.
-ex_elim h_dll_i12s1x2_5551.
+ex_elim h_dll_i12s1x2_5611.
 move=>[sigma_call1].
 subst.
-move=>H_dll_i12s1x2_5551.
+move=>H_dll_i12s1x2_5611.
 store_valid.
 ssl_read f.
 ssl_open.
-ssl_open_post H_dll_i12s1x2_5551.
-move=>[phi_dll_i12s1x2_55510].
-move=>[sigma_dll_i12s1x2_5551].
+ssl_open_post H_dll_i12s1x2_5611.
+move=>[phi_dll_i12s1x2_56110].
+move=>[sigma_dll_i12s1x2_5611].
 subst.
 ssl_alloc i2.
 ssl_dealloc x2.
@@ -155,13 +155,13 @@ exists (empty);
 sslauto.
 unfold_constructor 1;
 sslauto.
-ssl_open_post H_dll_i12s1x2_5551.
+ssl_open_post H_dll_i12s1x2_5611.
 ex_elim vi122 s1i12 wi122.
-ex_elim h_dll_wi122i12s1i12_552i12.
-move=>[phi_dll_i12s1x2_55510].
-move=>[sigma_dll_i12s1x2_5551].
+ex_elim h_dll_wi122i12s1i12_558i12.
+move=>[phi_dll_i12s1x2_56110].
+move=>[sigma_dll_i12s1x2_5611].
 subst.
-move=>H_dll_wi122i12s1i12_552i12.
+move=>H_dll_wi122i12s1i12_558i12.
 ssl_alloc i2.
 ssl_dealloc x2.
 ssl_dealloc (x2 .+ 1).
@@ -177,14 +177,14 @@ ssl_write i2.
 ssl_write_post i2.
 ssl_emp;
 exists (i2);
-exists (i2 :-> vx22 \+ i2 .+ 1 :-> i12 \+ i2 .+ 2 :-> null \+ i12 :-> vi122 \+ i12 .+ 1 :-> wi122 \+ i12 .+ 2 :-> i2 \+ h_dll_wi122i12s1i12_552i12);
+exists (i2 :-> vx22 \+ i2 .+ 1 :-> i12 \+ i2 .+ 2 :-> null \+ i12 :-> vi122 \+ i12 .+ 1 :-> wi122 \+ i12 .+ 2 :-> i2 \+ h_dll_wi122i12s1i12_558i12);
 sslauto.
 unfold_constructor 2;
 exists (vx22), ([:: vi122] ++ s1i12), (i12);
-exists (i12 :-> vi122 \+ i12 .+ 1 :-> wi122 \+ i12 .+ 2 :-> i2 \+ h_dll_wi122i12s1i12_552i12);
+exists (i12 :-> vi122 \+ i12 .+ 1 :-> wi122 \+ i12 .+ 2 :-> i2 \+ h_dll_wi122i12s1i12_558i12);
 sslauto.
 unfold_constructor 2;
 exists (vi122), (s1i12), (wi122);
-exists (h_dll_wi122i12s1i12_552i12);
+exists (h_dll_wi122i12s1i12_558i12);
 sslauto.
 Qed.
