examples/tree_copy.v
@@ -8,29 +8,29 @@ From SSL
 Require Import core.
 
 Inductive tree (x : ptr) (s : seq nat) (h : heap) : Prop :=
-| tree1 of x == null of
+| tree_1 of x == null of
   @perm_eq nat_eqType (s) (nil) /\ h = empty
-| tree2 of ~~ (x == null) of
+| tree_2 of (x == null) = false of
   exists (v : nat) (s1 : seq nat) (s2 : seq nat) (l : ptr) (r : ptr),
-  exists h_tree_ls1_523 h_tree_rs2_524,
-  @perm_eq nat_eqType (s) ([:: v] ++ s1 ++ s2) /\ h = x :-> v \+ x .+ 1 :-> l \+ x .+ 2 :-> r \+ h_tree_ls1_523 \+ h_tree_rs2_524 /\ tree l s1 h_tree_ls1_523 /\ tree r s2 h_tree_rs2_524.
+  exists h_tree_ls1_529 h_tree_rs2_530,
+  @perm_eq nat_eqType (s) ([:: v] ++ s1 ++ s2) /\ h = x :-> v \+ x .+ 1 :-> l \+ x .+ 2 :-> r \+ h_tree_ls1_529 \+ h_tree_rs2_530 /\ tree l s1 h_tree_ls1_529 /\ tree r s2 h_tree_rs2_530.
 
 Inductive treeN (x : ptr) (n : nat) (h : heap) : Prop :=
-| treeN1 of x == null of
+| treeN_1 of x == null of
   n == 0 /\ h = empty
-| treeN2 of ~~ (x == null) of
+| treeN_2 of (x == null) = false of
   exists (n1 : nat) (n2 : nat) (l : ptr) (r : ptr) (v : ptr),
-  exists h_treeN_ln1_525 h_treeN_rn2_526,
-  0 <= n1 /\ 0 <= n2 /\ n == 1 + n1 + n2 /\ h = x :-> v \+ x .+ 1 :-> l \+ x .+ 2 :-> r \+ h_treeN_ln1_525 \+ h_treeN_rn2_526 /\ treeN l n1 h_treeN_ln1_525 /\ treeN r n2 h_treeN_rn2_526.
+  exists h_treeN_ln1_531 h_treeN_rn2_532,
+  0 <= n1 /\ 0 <= n2 /\ n == 1 + n1 + n2 /\ h = x :-> v \+ x .+ 1 :-> l \+ x .+ 2 :-> r \+ h_treeN_ln1_531 \+ h_treeN_rn2_532 /\ treeN l n1 h_treeN_ln1_531 /\ treeN r n2 h_treeN_rn2_532.
 
-Lemma tree_perm_eq_trans12 x h s_1 s_2 : perm_eq s_1 s_2 -> tree x s_1 h -> tree x s_2 h. Admitted.
-Hint Resolve tree_perm_eq_trans12: ssl_pred.
-Lemma pure13 : @perm_eq nat_eqType (nil) (nil). Admitted.
-Hint Resolve pure13: ssl_pure.
-Lemma pure14 vx22 s1x2 s2x2 : @perm_eq nat_eqType ([:: vx22] ++ s1x2 ++ s2x2) ([:: vx22] ++ s1x2 ++ s2x2). Admitted.
-Hint Resolve pure14: ssl_pure.
-Lemma pure15 vx22 s1x2 s2x2 : @perm_eq nat_eqType ([:: vx22] ++ s1x2 ++ s2x2) ([:: vx22] ++ s1x2 ++ s2x2). Admitted.
-Hint Resolve pure15: ssl_pure.
+Lemma tree_perm_eq_trans19 x h s_1 s_2 : perm_eq s_1 s_2 -> tree x s_1 h -> tree x s_2 h. Admitted.
+Hint Resolve tree_perm_eq_trans19: ssl_pred.
+Lemma pure20 : @perm_eq nat_eqType (nil) (nil). Admitted.
+Hint Resolve pure20: ssl_pure.
+Lemma pure21 vx22 s1x2 s2x2 : @perm_eq nat_eqType ([:: vx22] ++ s1x2 ++ s2x2) ([:: vx22] ++ s1x2 ++ s2x2). Admitted.
+Hint Resolve pure21: ssl_pure.
+Lemma pure22 vx22 s1x2 s2x2 : @perm_eq nat_eqType ([:: vx22] ++ s1x2 ++ s2x2) ([:: vx22] ++ s1x2 ++ s2x2). Admitted.
+Hint Resolve pure22: ssl_pure.
 
 Definition tree_copy_type :=
   forall (vprogs : ptr),
@@ -100,38 +100,38 @@ unfold_constructor 1;
 sslauto.
 ssl_open_post H_tree_x2s_a.
 ex_elim vx22 s1x2 s2x2 lx22 rx22.
-ex_elim h_tree_lx22s1x2_523x2 h_tree_rx22s2x2_524x2.
+ex_elim h_tree_lx22s1x2_529x2 h_tree_rx22s2x2_530x2.
 move=>[phi_tree_x2s_a0].
 move=>[sigma_tree_x2s_a].
 subst.
-move=>[H_tree_lx22s1x2_523x2 H_tree_rx22s2x2_524x2].
+move=>[H_tree_lx22s1x2_529x2 H_tree_rx22s2x2_530x2].
 ssl_read x2.
 ssl_read (x2 .+ 1).
 ssl_read (x2 .+ 2).
 ssl_write r.
-ssl_call_pre (r :-> lx22 \+ h_tree_lx22s1x2_523x2).
+ssl_call_pre (r :-> lx22 \+ h_tree_lx22s1x2_529x2).
 ssl_call (lx22, s1x2).
-exists (h_tree_lx22s1x2_523x2);
+exists (h_tree_lx22s1x2_529x2);
 sslauto.
 move=>h_call1.
 ex_elim y12.
-ex_elim h_tree_lx22s1x2_523x2 h_tree_y12s1x2_523x2.
+ex_elim h_tree_lx22s1x2_529x2 h_tree_y12s1x2_529x2.
 move=>[sigma_call1].
 subst.
-move=>[H_tree_lx22s1x2_523x2 H_tree_y12s1x2_523x2].
+move=>[H_tree_lx22s1x2_529x2 H_tree_y12s1x2_529x2].
 store_valid.
 ssl_read r.
 ssl_write r.
-ssl_call_pre (r :-> rx22 \+ h_tree_rx22s2x2_524x2).
+ssl_call_pre (r :-> rx22 \+ h_tree_rx22s2x2_530x2).
 ssl_call (rx22, s2x2).
-exists (h_tree_rx22s2x2_524x2);
+exists (h_tree_rx22s2x2_530x2);
 sslauto.
 move=>h_call2.
 ex_elim y22.
-ex_elim h_tree_rx22s2x2_524x2 h_tree_y22s2x2_524x2.
+ex_elim h_tree_rx22s2x2_530x2 h_tree_y22s2x2_530x2.
 move=>[sigma_call2].
 subst.
-move=>[H_tree_rx22s2x2_524x2 H_tree_y22s2x2_524x2].
+move=>[H_tree_rx22s2x2_530x2 H_tree_y22s2x2_530x2].
 store_valid.
 ssl_read r.
 ssl_alloc y3.
@@ -145,17 +145,17 @@ ssl_write y3.
 ssl_write_post y3.
 ssl_emp;
 exists (y3);
-exists (x2 :-> vx22 \+ x2 .+ 1 :-> lx22 \+ x2 .+ 2 :-> rx22 \+ h_tree_lx22s1x2_523x2 \+ h_tree_rx22s2x2_524x2);
-exists (y3 :-> vx22 \+ y3 .+ 1 :-> y12 \+ y3 .+ 2 :-> y22 \+ h_tree_y12s1x2_523x2 \+ h_tree_y22s2x2_524x2);
+exists (x2 :-> vx22 \+ x2 .+ 1 :-> lx22 \+ x2 .+ 2 :-> rx22 \+ h_tree_lx22s1x2_529x2 \+ h_tree_rx22s2x2_530x2);
+exists (y3 :-> vx22 \+ y3 .+ 1 :-> y12 \+ y3 .+ 2 :-> y22 \+ h_tree_y12s1x2_529x2 \+ h_tree_y22s2x2_530x2);
 sslauto.
 unfold_constructor 2;
 exists (vx22), (s1x2), (s2x2), (lx22), (rx22);
-exists (h_tree_lx22s1x2_523x2);
-exists (h_tree_rx22s2x2_524x2);
+exists (h_tree_lx22s1x2_529x2);
+exists (h_tree_rx22s2x2_530x2);
 sslauto.
 unfold_constructor 2;
 exists (vx22), (s1x2), (s2x2), (y12), (y22);
-exists (h_tree_y12s1x2_523x2);
-exists (h_tree_y22s2x2_524x2);
+exists (h_tree_y12s1x2_529x2);
+exists (h_tree_y22s2x2_530x2);
 sslauto.
 Qed.
