examples/tree_free.v
@@ -8,23 +8,23 @@ From SSL
 Require Import core.
 
 Inductive tree (x : ptr) (s : seq nat) (h : heap) : Prop :=
-| tree1 of x == null of
+| tree_1 of x == null of
   @perm_eq nat_eqType (s) (nil) /\ h = empty
-| tree2 of ~~ (x == null) of
+| tree_2 of (x == null) = false of
   exists (v : nat) (s1 : seq nat) (s2 : seq nat) (l : ptr) (r : ptr),
-  exists h_tree_ls1_527 h_tree_rs2_528,
-  @perm_eq nat_eqType (s) ([:: v] ++ s1 ++ s2) /\ h = x :-> v \+ x .+ 1 :-> l \+ x .+ 2 :-> r \+ h_tree_ls1_527 \+ h_tree_rs2_528 /\ tree l s1 h_tree_ls1_527 /\ tree r s2 h_tree_rs2_528.
+  exists h_tree_ls1_533 h_tree_rs2_534,
+  @perm_eq nat_eqType (s) ([:: v] ++ s1 ++ s2) /\ h = x :-> v \+ x .+ 1 :-> l \+ x .+ 2 :-> r \+ h_tree_ls1_533 \+ h_tree_rs2_534 /\ tree l s1 h_tree_ls1_533 /\ tree r s2 h_tree_rs2_534.
 
 Inductive treeN (x : ptr) (n : nat) (h : heap) : Prop :=
-| treeN1 of x == null of
+| treeN_1 of x == null of
   n == 0 /\ h = empty
-| treeN2 of ~~ (x == null) of
+| treeN_2 of (x == null) = false of
   exists (n1 : nat) (n2 : nat) (l : ptr) (r : ptr) (v : ptr),
-  exists h_treeN_ln1_529 h_treeN_rn2_530,
-  0 <= n1 /\ 0 <= n2 /\ n == 1 + n1 + n2 /\ h = x :-> v \+ x .+ 1 :-> l \+ x .+ 2 :-> r \+ h_treeN_ln1_529 \+ h_treeN_rn2_530 /\ treeN l n1 h_treeN_ln1_529 /\ treeN r n2 h_treeN_rn2_530.
+  exists h_treeN_ln1_535 h_treeN_rn2_536,
+  0 <= n1 /\ 0 <= n2 /\ n == 1 + n1 + n2 /\ h = x :-> v \+ x .+ 1 :-> l \+ x .+ 2 :-> r \+ h_treeN_ln1_535 \+ h_treeN_rn2_536 /\ treeN l n1 h_treeN_ln1_535 /\ treeN r n2 h_treeN_rn2_536.
 
-Lemma tree_perm_eq_trans16 x h s_1 s_2 : perm_eq s_1 s_2 -> tree x s_1 h -> tree x s_2 h. Admitted.
-Hint Resolve tree_perm_eq_trans16: ssl_pred.
+Lemma tree_perm_eq_trans23 x h s_1 s_2 : perm_eq s_1 s_2 -> tree x s_1 h -> tree x s_2 h. Admitted.
+Hint Resolve tree_perm_eq_trans23: ssl_pred.
 
 Definition tree_free_type :=
   forall (vprogs : ptr),
@@ -33,8 +33,8 @@ Definition tree_free_type :=
     fun h =>
       let: (x) := vprogs in
       let: (s) := vghosts in
-      exists h_tree_xs_531,
-      h = h_tree_xs_531 /\ tree x s h_tree_xs_531,
+      exists h_tree_xs_537,
+      h = h_tree_xs_537 /\ tree x s h_tree_xs_537,
     [vfun (_: unit) h =>
       let: (x) := vprogs in
       let: (s) := vghosts in
@@ -62,38 +62,38 @@ Obligation Tactic := intro; move=>x; ssl_program_simpl.
 Next Obligation.
 ssl_ghostelim_pre.
 move=>s.
-ex_elim h_tree_xs_531.
+ex_elim h_tree_xs_537.
 move=>[sigma_self].
 subst.
-move=>H_tree_xs_531.
+move=>H_tree_xs_537.
 ssl_ghostelim_post.
 ssl_open.
-ssl_open_post H_tree_xs_531.
-move=>[phi_tree_xs_5310].
-move=>[sigma_tree_xs_531].
+ssl_open_post H_tree_xs_537.
+move=>[phi_tree_xs_5370].
+move=>[sigma_tree_xs_537].
 subst.
 ssl_emp;
 sslauto.
-ssl_open_post H_tree_xs_531.
+ssl_open_post H_tree_xs_537.
 ex_elim vx2 s1x s2x lx2 rx2.
-ex_elim h_tree_lx2s1x_527x h_tree_rx2s2x_528x.
-move=>[phi_tree_xs_5310].
-move=>[sigma_tree_xs_531].
+ex_elim h_tree_lx2s1x_533x h_tree_rx2s2x_534x.
+move=>[phi_tree_xs_5370].
+move=>[sigma_tree_xs_537].
 subst.
-move=>[H_tree_lx2s1x_527x H_tree_rx2s2x_528x].
+move=>[H_tree_lx2s1x_533x H_tree_rx2s2x_534x].
 ssl_read (x .+ 1).
 ssl_read (x .+ 2).
-ssl_call_pre (h_tree_lx2s1x_527x).
+ssl_call_pre (h_tree_lx2s1x_533x).
 ssl_call (s1x).
-exists (h_tree_lx2s1x_527x);
+exists (h_tree_lx2s1x_533x);
 sslauto.
 move=>h_call1.
 move=>[sigma_call1].
 subst.
 store_valid.
-ssl_call_pre (h_tree_rx2s2x_528x).
+ssl_call_pre (h_tree_rx2s2x_534x).
 ssl_call (s2x).
-exists (h_tree_rx2s2x_528x);
+exists (h_tree_rx2s2x_534x);
 sslauto.
 move=>h_call2.
 move=>[sigma_call2].
