examples/tree_size.v
@@ -8,27 +8,27 @@ From SSL
 Require Import core.
 
 Inductive tree (x : ptr) (s : seq nat) (h : heap) : Prop :=
-| tree1 of x == null of
+| tree_1 of x == null of
   @perm_eq nat_eqType (s) (nil) /\ h = empty
-| tree2 of ~~ (x == null) of
+| tree_2 of (x == null) = false of
   exists (v : nat) (s1 : seq nat) (s2 : seq nat) (l : ptr) (r : ptr),
-  exists h_tree_ls1_519 h_tree_rs2_520,
-  @perm_eq nat_eqType (s) ([:: v] ++ s1 ++ s2) /\ h = x :-> v \+ x .+ 1 :-> l \+ x .+ 2 :-> r \+ h_tree_ls1_519 \+ h_tree_rs2_520 /\ tree l s1 h_tree_ls1_519 /\ tree r s2 h_tree_rs2_520.
+  exists h_tree_ls1_525 h_tree_rs2_526,
+  @perm_eq nat_eqType (s) ([:: v] ++ s1 ++ s2) /\ h = x :-> v \+ x .+ 1 :-> l \+ x .+ 2 :-> r \+ h_tree_ls1_525 \+ h_tree_rs2_526 /\ tree l s1 h_tree_ls1_525 /\ tree r s2 h_tree_rs2_526.
 
 Inductive treeN (x : ptr) (n : nat) (h : heap) : Prop :=
-| treeN1 of x == null of
+| treeN_1 of x == null of
   n == 0 /\ h = empty
-| treeN2 of ~~ (x == null) of
+| treeN_2 of (x == null) = false of
   exists (n1 : nat) (n2 : nat) (l : ptr) (r : ptr) (v : ptr),
-  exists h_treeN_ln1_521 h_treeN_rn2_522,
-  0 <= n1 /\ 0 <= n2 /\ n == 1 + n1 + n2 /\ h = x :-> v \+ x .+ 1 :-> l \+ x .+ 2 :-> r \+ h_treeN_ln1_521 \+ h_treeN_rn2_522 /\ treeN l n1 h_treeN_ln1_521 /\ treeN r n2 h_treeN_rn2_522.
+  exists h_treeN_ln1_527 h_treeN_rn2_528,
+  0 <= n1 /\ 0 <= n2 /\ n == 1 + n1 + n2 /\ h = x :-> v \+ x .+ 1 :-> l \+ x .+ 2 :-> r \+ h_treeN_ln1_527 \+ h_treeN_rn2_528 /\ treeN l n1 h_treeN_ln1_527 /\ treeN r n2 h_treeN_rn2_528.
 
-Lemma tree_perm_eq_trans9 x h s_1 s_2 : perm_eq s_1 s_2 -> tree x s_1 h -> tree x s_2 h. Admitted.
-Hint Resolve tree_perm_eq_trans9: ssl_pred.
-Lemma pure10 : 0 == 0. Admitted.
-Hint Resolve pure10: ssl_pure.
-Lemma pure11 n1x2 n2x2 : 0 <= 1 + n1x2 + n2x2 -> 0 <= n2x2 -> 0 <= n1x2 -> 1 + n1x2 + n2x2 == 1 + n1x2 + n2x2. Admitted.
-Hint Resolve pure11: ssl_pure.
+Lemma tree_perm_eq_trans16 x h s_1 s_2 : perm_eq s_1 s_2 -> tree x s_1 h -> tree x s_2 h. Admitted.
+Hint Resolve tree_perm_eq_trans16: ssl_pred.
+Lemma pure17 : 0 == 0. Admitted.
+Hint Resolve pure17: ssl_pure.
+Lemma pure18 n1x2 n2x2 : 0 <= n1x2 -> 0 <= n2x2 -> 0 <= 1 + n1x2 + n2x2 -> 1 + n1x2 + n2x2 == 1 + n1x2 + n2x2. Admitted.
+Hint Resolve pure18: ssl_pure.
 
 Definition tree_size_type :=
   forall (vprogs : ptr * ptr),
@@ -86,44 +86,44 @@ unfold_constructor 1;
 sslauto.
 ssl_open_post H_treeN_xn_a.
 ex_elim n1x2 n2x2 lx2 rx2 vx2.
-ex_elim h_treeN_lx2n1x2_521x h_treeN_rx2n2x2_522x.
+ex_elim h_treeN_lx2n1x2_527x h_treeN_rx2n2x2_528x.
 move=>[phi_treeN_xn_a0] [phi_treeN_xn_a1] [phi_treeN_xn_a2].
 move=>[sigma_treeN_xn_a].
 subst.
-move=>[H_treeN_lx2n1x2_521x H_treeN_rx2n2x2_522x].
+move=>[H_treeN_lx2n1x2_527x H_treeN_rx2n2x2_528x].
 ssl_read (x .+ 1).
 ssl_read (x .+ 2).
-ssl_call_pre (r :-> 0 \+ h_treeN_lx2n1x2_521x).
+ssl_call_pre (r :-> 0 \+ h_treeN_lx2n1x2_527x).
 ssl_call (n1x2).
-exists (h_treeN_lx2n1x2_521x);
+exists (h_treeN_lx2n1x2_527x);
 sslauto.
 move=>h_call1.
-ex_elim h_treeN_lx2n1x2_521x.
+ex_elim h_treeN_lx2n1x2_527x.
 move=>[sigma_call1].
 subst.
-move=>H_treeN_lx2n1x2_521x.
+move=>H_treeN_lx2n1x2_527x.
 store_valid.
 ssl_read r.
 ssl_write r.
-ssl_call_pre (r :-> 0 \+ h_treeN_rx2n2x2_522x).
+ssl_call_pre (r :-> 0 \+ h_treeN_rx2n2x2_528x).
 ssl_call (n2x2).
-exists (h_treeN_rx2n2x2_522x);
+exists (h_treeN_rx2n2x2_528x);
 sslauto.
 move=>h_call2.
-ex_elim h_treeN_rx2n2x2_522x.
+ex_elim h_treeN_rx2n2x2_528x.
 move=>[sigma_call2].
 subst.
-move=>H_treeN_rx2n2x2_522x.
+move=>H_treeN_rx2n2x2_528x.
 store_valid.
 ssl_read r.
 ssl_write r.
 ssl_write_post r.
 ssl_emp;
-exists (x :-> vx2 \+ x .+ 1 :-> lx2 \+ x .+ 2 :-> rx2 \+ h_treeN_lx2n1x2_521x \+ h_treeN_rx2n2x2_522x);
+exists (x :-> vx2 \+ x .+ 1 :-> lx2 \+ x .+ 2 :-> rx2 \+ h_treeN_lx2n1x2_527x \+ h_treeN_rx2n2x2_528x);
 sslauto.
 unfold_constructor 2;
 exists (n1x2), (n2x2), (lx2), (rx2), (vx2);
-exists (h_treeN_lx2n1x2_521x);
-exists (h_treeN_rx2n2x2_522x);
+exists (h_treeN_lx2n1x2_527x);
+exists (h_treeN_rx2n2x2_528x);
 sslauto.
 Qed.
