examples/bst_insert.v
@@ -1,0 +1,199 @@
+From mathcomp
+Require Import ssreflect ssrbool ssrnat eqtype seq ssrfun.
+From fcsl
+Require Import prelude pred pcm unionmap heap.
+From HTT
+Require Import stmod stsep stlog stlogR.
+From SSL
+Require Import core.
+
+Inductive bst (x : ptr) (sz : nat) (lo : nat) (hi : nat) (h : heap) : Prop :=
+| bst_1 of x == null of
+  hi == 0 /\ lo == 7 /\ sz == 0 /\ h = empty
+| bst_2 of (x == null) = false of
+  exists (sz1 : nat) (sz2 : nat) (v : nat) (hi2 : nat) (hi1 : nat) (lo1 : nat) (lo2 : nat) (l : ptr) (r : ptr),
+  exists h_bst_lsz1lo1hi1_513 h_bst_rsz2lo2hi2_514,
+  0 <= sz1 /\ 0 <= sz2 /\ 0 <= v /\ hi == (if hi2 <= v then v else hi2) /\ hi1 <= v /\ lo == (if v <= lo1 then v else lo1) /\ sz == 1 + sz1 + sz2 /\ v <= 7 /\ v <= lo2 /\ h = x :-> v \+ x .+ 1 :-> l \+ x .+ 2 :-> r \+ h_bst_lsz1lo1hi1_513 \+ h_bst_rsz2lo2hi2_514 /\ bst l sz1 lo1 hi1 h_bst_lsz1lo1hi1_513 /\ bst r sz2 lo2 hi2 h_bst_rsz2lo2hi2_514.
+
+Lemma pure1 : 0 <= 0. Admitted.
+Hint Resolve pure1: ssl_pure.
+Lemma pure2 : 1 == 1. Admitted.
+Hint Resolve pure2: ssl_pure.
+Lemma pure3 a : a < a + 3. Admitted.
+Hint Resolve pure3: ssl_pure.
+Lemma pure4 k2 : k2 <= 7 -> 0 <= k2 -> (if k2 <= 7 then k2 else 7) == (if k2 <= 7 then k2 else 7). Admitted.
+Hint Resolve pure4: ssl_pure.
+Lemma pure5 k2 : k2 <= 7 -> 0 <= k2 -> (if 0 <= k2 then k2 else 0) == (if 0 <= k2 then k2 else 0). Admitted.
+Hint Resolve pure5: ssl_pure.
+Lemma pure6 sz1x sz2x : 0 <= 1 + sz1x + sz2x -> 0 <= sz2x -> 0 <= sz1x -> 0 <= sz1x + 1. Admitted.
+Hint Resolve pure6: ssl_pure.
+Lemma pure7 sz1x sz2x : 0 <= 1 + sz1x + sz2x -> 0 <= sz1x -> 0 <= sz2x -> 1 + sz1x + sz2x + 1 == 1 + sz1x + 1 + sz2x. Admitted.
+Hint Resolve pure7: ssl_pure.
+Lemma pure8 hi1x k2 vx2 lo2x : hi1x <= vx2 -> vx2 <= lo2x -> k2 <= vx2 -> 0 <= vx2 -> vx2 <= 7 -> 0 <= k2 -> k2 <= 7 -> (if hi1x <= k2 then k2 else hi1x) <= vx2. Admitted.
+Hint Resolve pure8: ssl_pure.
+Lemma pure9 k2 lo2x hi1x vx2 lo1x : hi1x <= vx2 -> vx2 <= lo2x -> k2 <= vx2 -> 0 <= vx2 -> vx2 <= 7 -> 0 <= k2 -> k2 <= 7 -> (if k2 <= (if vx2 <= lo1x then vx2 else lo1x) then k2 else (if vx2 <= lo1x then vx2 else lo1x)) == (if vx2 <= (if k2 <= lo1x then k2 else lo1x) then vx2 else (if k2 <= lo1x then k2 else lo1x)). Admitted.
+Hint Resolve pure9: ssl_pure.
+Lemma pure10 k2 hi2x lo2x hi1x vx2 : hi1x <= vx2 -> vx2 <= lo2x -> k2 <= vx2 -> 0 <= vx2 -> vx2 <= 7 -> 0 <= k2 -> k2 <= 7 -> (if (if hi2x <= vx2 then vx2 else hi2x) <= k2 then k2 else (if hi2x <= vx2 then vx2 else hi2x)) == (if hi2x <= vx2 then vx2 else hi2x). Admitted.
+Hint Resolve pure10: ssl_pure.
+Lemma pure11 sz1x sz2x : 0 <= 1 + sz1x + sz2x -> 0 <= sz1x -> 0 <= sz2x -> 1 + sz1x + sz2x + 1 == 1 + sz1x + sz2x + 1. Admitted.
+Hint Resolve pure11: ssl_pure.
+Lemma pure12 sz2x sz1x : 0 <= 1 + sz1x + sz2x -> 0 <= sz1x -> 0 <= sz2x -> 0 <= sz2x + 1. Admitted.
+Hint Resolve pure12: ssl_pure.
+Lemma pure13 k2 lo2x hi1x vx2 lo1x : hi1x <= vx2 -> vx2 <= lo2x -> 0 <= vx2 -> vx2 <= 7 -> 0 <= k2 -> k2 <= 7 -> (k2 <= vx2) = false -> (if k2 <= (if vx2 <= lo1x then vx2 else lo1x) then k2 else (if vx2 <= lo1x then vx2 else lo1x)) == (if vx2 <= lo1x then vx2 else lo1x). Admitted.
+Hint Resolve pure13: ssl_pure.
+Lemma pure14 vx2 k2 lo2x hi1x : hi1x <= vx2 -> vx2 <= lo2x -> 0 <= vx2 -> vx2 <= 7 -> 0 <= k2 -> k2 <= 7 -> (k2 <= vx2) = false -> vx2 <= (if k2 <= lo2x then k2 else lo2x). Admitted.
+Hint Resolve pure14: ssl_pure.
+Lemma pure15 k2 hi2x lo2x hi1x vx2 : hi1x <= vx2 -> vx2 <= lo2x -> 0 <= vx2 -> vx2 <= 7 -> 0 <= k2 -> k2 <= 7 -> (k2 <= vx2) = false -> (if (if hi2x <= vx2 then vx2 else hi2x) <= k2 then k2 else (if hi2x <= vx2 then vx2 else hi2x)) == (if (if hi2x <= k2 then k2 else hi2x) <= vx2 then vx2 else (if hi2x <= k2 then k2 else hi2x)). Admitted.
+Hint Resolve pure15: ssl_pure.
+
+Definition bst_insert_type :=
+  forall (vprogs : ptr * ptr),
+  {(vghosts : nat * nat * nat * nat)},
+  STsep (
+    fun h =>
+      let: (x, retv) := vprogs in
+      let: (k, n, lo, hi) := vghosts in
+      exists h_bst_xnlohi_a,
+      0 <= k /\ 0 <= n /\ k <= 7 /\ h = retv :-> k \+ h_bst_xnlohi_a /\ bst x n lo hi h_bst_xnlohi_a,
+    [vfun (_: unit) h =>
+      let: (x, retv) := vprogs in
+      let: (k, n, lo, hi) := vghosts in
+      exists hi1 lo1 n1 y,
+      exists h_bst_yn1lo1hi1_b,
+      hi1 == (if hi <= k then k else hi) /\ lo1 == (if k <= lo then k else lo) /\ n1 == n + 1 /\ h = retv :-> y \+ h_bst_yn1lo1hi1_b /\ bst y n1 lo1 hi1 h_bst_yn1lo1hi1_b
+    ]).
+
+Program Definition bst_insert : bst_insert_type :=
+  Fix (fun (bst_insert : bst_insert_type) vprogs =>
+    let: (x, retv) := vprogs in
+    Do (
+      k2 <-- @read nat retv;
+      if x == null
+      then
+        y2 <-- allocb null 3;
+        retv ::= y2;;
+        (y2 .+ 1) ::= null;;
+        (y2 .+ 2) ::= null;;
+        y2 ::= k2;;
+        ret tt
+      else
+        vx2 <-- @read nat x;
+        if k2 <= vx2
+        then
+          lx2 <-- @read ptr (x .+ 1);
+          bst_insert (lx2, retv);;
+          y12 <-- @read ptr retv;
+          (x .+ 1) ::= y12;;
+          retv ::= x;;
+          ret tt
+        else
+          rx2 <-- @read ptr (x .+ 2);
+          bst_insert (rx2, retv);;
+          y12 <-- @read ptr retv;
+          (x .+ 2) ::= y12;;
+          retv ::= x;;
+          ret tt
+    )).
+Obligation Tactic := intro; move=>[x retv]; ssl_program_simpl.
+Next Obligation.
+ssl_ghostelim_pre.
+move=>[[[k2 n] lo] hi].
+ex_elim h_bst_xnlohi_a.
+move=>[phi_self0] [phi_self1] [phi_self2].
+move=>[sigma_self].
+subst.
+move=>H_bst_xnlohi_a.
+ssl_ghostelim_post.
+ssl_read retv.
+ssl_open.
+ssl_open_post H_bst_xnlohi_a.
+move=>[phi_bst_xnlohi_a0] [phi_bst_xnlohi_a1] [phi_bst_xnlohi_a2].
+move=>[sigma_bst_xnlohi_a].
+subst.
+ssl_alloc y2.
+ssl_write retv.
+ssl_write_post retv.
+ssl_write (y2 .+ 1).
+ssl_write_post (y2 .+ 1).
+ssl_write (y2 .+ 2).
+ssl_write_post (y2 .+ 2).
+ssl_write y2.
+ssl_write_post y2.
+ssl_emp;
+exists ((if 0 <= k2 then k2 else 0)), ((if k2 <= 7 then k2 else 7)), (0 + 1), (y2);
+exists (y2 :-> k2 \+ y2 .+ 1 :-> null \+ y2 .+ 2 :-> null);
+sslauto.
+unfold_constructor 2;
+exists (0), (0), (k2), (0), (0), (7), (7), (null), (null);
+exists (empty);
+exists (empty);
+sslauto.
+unfold_constructor 1;
+sslauto.
+unfold_constructor 1;
+sslauto.
+ssl_open_post H_bst_xnlohi_a.
+ex_elim sz1x sz2x vx2 hi2x hi1x.
+ex_elim lo1x lo2x lx2 rx2.
+ex_elim h_bst_lx2sz1xlo1xhi1x_513x h_bst_rx2sz2xlo2xhi2x_514x.
+move=>[phi_bst_xnlohi_a0] [phi_bst_xnlohi_a1] [phi_bst_xnlohi_a2] [phi_bst_xnlohi_a3] [phi_bst_xnlohi_a4] [phi_bst_xnlohi_a5] [phi_bst_xnlohi_a6] [phi_bst_xnlohi_a7] [phi_bst_xnlohi_a8].
+move=>[sigma_bst_xnlohi_a].
+subst.
+move=>[H_bst_lx2sz1xlo1xhi1x_513x H_bst_rx2sz2xlo2xhi2x_514x].
+ssl_read x.
+ssl_abduce_branch.
+ssl_read (x .+ 1).
+ssl_call_pre (retv :-> k2 \+ h_bst_lx2sz1xlo1xhi1x_513x).
+ssl_call (k2, sz1x, lo1x, hi1x).
+exists (h_bst_lx2sz1xlo1xhi1x_513x);
+sslauto.
+move=>h_call1.
+ex_elim hi11 lo11 n11 y12.
+ex_elim h_bst_y12sz1xk2lo1xk2lo1xhi1xk2k2hi1x_513x.
+move=>[phi_call10] [phi_call11] [phi_call12].
+move=>[sigma_call1].
+subst.
+move=>H_bst_y12n11lo11hi11_b1.
+store_valid.
+ssl_read retv.
+ssl_write (x .+ 1).
+ssl_write_post (x .+ 1).
+ssl_write retv.
+ssl_write_post retv.
+ssl_emp;
+exists ((if (if hi2x <= vx2 then vx2 else hi2x) <= k2 then k2 else (if hi2x <= vx2 then vx2 else hi2x))), ((if k2 <= (if vx2 <= lo1x then vx2 else lo1x) then k2 else (if vx2 <= lo1x then vx2 else lo1x))), (1 + sz1x + sz2x + 1), (x);
+exists (x :-> vx2 \+ x .+ 1 :-> y12 \+ x .+ 2 :-> rx2 \+ h_bst_y12sz1xk2lo1xk2lo1xhi1xk2k2hi1x_513x \+ h_bst_rx2sz2xlo2xhi2x_514x);
+sslauto.
+unfold_constructor 2;
+exists (sz1x + 1), (sz2x), (vx2), (hi2x), ((if hi1x <= k2 then k2 else hi1x)), ((if k2 <= lo1x then k2 else lo1x)), (lo2x), (y12), (rx2);
+exists (h_bst_y12sz1xk2lo1xk2lo1xhi1xk2k2hi1x_513x);
+exists (h_bst_rx2sz2xlo2xhi2x_514x);
+sslauto.
+ssl_read (x .+ 2).
+ssl_call_pre (retv :-> k2 \+ h_bst_rx2sz2xlo2xhi2x_514x).
+ssl_call (k2, sz2x, lo2x, hi2x).
+exists (h_bst_rx2sz2xlo2xhi2x_514x);
+sslauto.
+move=>h_call2.
+ex_elim hi11 lo11 n11 y12.
+ex_elim h_bst_y12sz2xk2lo2xk2lo2xhi2xk2k2hi2x_514x.
+move=>[phi_call20] [phi_call21] [phi_call22].
+move=>[sigma_call2].
+subst.
+move=>H_bst_y12n11lo11hi11_b1.
+store_valid.
+ssl_read retv.
+ssl_write (x .+ 2).
+ssl_write_post (x .+ 2).
+ssl_write retv.
+ssl_write_post retv.
+ssl_emp;
+exists ((if (if hi2x <= vx2 then vx2 else hi2x) <= k2 then k2 else (if hi2x <= vx2 then vx2 else hi2x))), ((if k2 <= (if vx2 <= lo1x then vx2 else lo1x) then k2 else (if vx2 <= lo1x then vx2 else lo1x))), (1 + sz1x + sz2x + 1), (x);
+exists (x :-> vx2 \+ x .+ 1 :-> lx2 \+ x .+ 2 :-> y12 \+ h_bst_lx2sz1xlo1xhi1x_513x \+ h_bst_y12sz2xk2lo2xk2lo2xhi2xk2k2hi2x_514x);
+sslauto.
+unfold_constructor 2;
+exists (sz1x), (sz2x + 1), (vx2), ((if hi2x <= k2 then k2 else hi2x)), (hi1x), (lo1x), ((if k2 <= lo2x then k2 else lo2x)), (lx2), (y12);
+exists (h_bst_lx2sz1xlo1xhi1x_513x);
+exists (h_bst_y12sz2xk2lo2xk2lo2xhi2xk2k2hi2x_514x);
+sslauto.
+Qed.
