examples/bst_left_rotate.v
@@ -8,9 +8,9 @@ From SSL
 Require Import core.
 
 Inductive bst (x : ptr) (sz : nat) (lo : nat) (hi : nat) (h : heap) : Prop :=
-| bst1 of x == null of
+| bst_1 of x == null of
   hi == 0 /\ lo == 7 /\ sz == 0 /\ h = empty
-| bst2 of ~~ (x == null) of
+| bst_2 of (x == null) = false of
   exists (sz1 : nat) (sz2 : nat) (v : nat) (hi2 : nat) (hi1 : nat) (lo1 : nat) (lo2 : nat) (l : ptr) (r : ptr),
   exists h_bst_lsz1lo1hi1_513 h_bst_rsz2lo2hi2_514,
   0 <= sz1 /\ 0 <= sz2 /\ 0 <= v /\ hi == (if hi2 <= v then v else hi2) /\ hi1 <= v /\ lo == (if v <= lo1 then v else lo1) /\ sz == 1 + sz1 + sz2 /\ v <= 7 /\ v <= lo2 /\ h = x :-> v \+ x .+ 1 :-> l \+ x .+ 2 :-> r \+ h_bst_lsz1lo1hi1_513 \+ h_bst_rsz2lo2hi2_514 /\ bst l sz1 lo1 hi1 h_bst_lsz1lo1hi1_513 /\ bst r sz2 lo2 hi2 h_bst_rsz2lo2hi2_514.
@@ -19,9 +19,9 @@ Lemma pure1 sz1 sz1r2 sz2r2 : 0 <= sz1 -> 0 <= 1 + sz1r2 + sz2r2 -> 0 <= sz2r2 -
 Hint Resolve pure1: ssl_pure.
 Lemma pure2 sz1 sz1r2 sz2r2 : 0 <= sz1 -> 0 <= 1 + sz1r2 + sz2r2 -> 0 <= sz2r2 -> 0 <= sz1r2 -> 1 + sz1 + sz1r2 + sz2r2 == sz1 + 1 + sz1r2 + sz2r2. Admitted.
 Hint Resolve pure2: ssl_pure.
-Lemma pure3 lo1r2 vr22 hi1 v2 hi1r2 lo2r2 : vr22 <= 7 -> v2 <= (if vr22 <= lo1r2 then vr22 else lo1r2) -> 0 <= v2 -> vr22 <= lo2r2 -> 0 <= vr22 -> hi1r2 <= vr22 -> hi1 <= v2 -> v2 <= 7 -> (if hi1r2 <= v2 then v2 else hi1r2) <= vr22. Admitted.
+Lemma pure3 lo1r2 vr22 hi1 v2 hi1r2 lo2r2 : vr22 <= 7 -> v2 <= (if vr22 <= lo1r2 then vr22 else lo1r2) -> 0 <= v2 -> vr22 <= lo2r2 -> 0 <= vr22 -> hi1r2 <= vr22 -> hi1 <= v2 -> v2 <= 7 -> v2 <= lo1r2. Admitted.
 Hint Resolve pure3: ssl_pure.
-Lemma pure4 lo1r2 vr22 hi1 v2 hi1r2 lo2r2 : vr22 <= 7 -> v2 <= (if vr22 <= lo1r2 then vr22 else lo1r2) -> 0 <= v2 -> vr22 <= lo2r2 -> 0 <= vr22 -> hi1r2 <= vr22 -> hi1 <= v2 -> v2 <= 7 -> v2 <= lo1r2. Admitted.
+Lemma pure4 lo1r2 vr22 hi1 v2 hi1r2 lo2r2 : vr22 <= 7 -> v2 <= (if vr22 <= lo1r2 then vr22 else lo1r2) -> 0 <= v2 -> vr22 <= lo2r2 -> 0 <= vr22 -> hi1r2 <= vr22 -> hi1 <= v2 -> v2 <= 7 -> (if hi1r2 <= v2 then v2 else hi1r2) <= vr22. Admitted.
 Hint Resolve pure4: ssl_pure.
 
 Definition bst_left_rotate_type :=
@@ -32,7 +32,7 @@ Definition bst_left_rotate_type :=
       let: (x, retv) := vprogs in
       let: (sz1, sz2, v, hi1, r, lo2, l, lo1, hi2, unused) := vghosts in
       exists h_bst_lsz1lo1hi1_a h_bst_rsz2lo2hi2_b,
-      0 <= sz1 /\ 0 <= sz2 /\ 0 <= v /\ hi1 <= v /\ ~~ (r == null) /\ v <= 7 /\ v <= lo2 /\ h = retv :-> unused \+ x :-> v \+ x .+ 1 :-> l \+ x .+ 2 :-> r \+ h_bst_lsz1lo1hi1_a \+ h_bst_rsz2lo2hi2_b /\ bst l sz1 lo1 hi1 h_bst_lsz1lo1hi1_a /\ bst r sz2 lo2 hi2 h_bst_rsz2lo2hi2_b,
+      0 <= sz1 /\ 0 <= sz2 /\ 0 <= v /\ hi1 <= v /\ (r == null) = false /\ v <= 7 /\ v <= lo2 /\ h = retv :-> unused \+ x :-> v \+ x .+ 1 :-> l \+ x .+ 2 :-> r \+ h_bst_lsz1lo1hi1_a \+ h_bst_rsz2lo2hi2_b /\ bst l sz1 lo1 hi1 h_bst_lsz1lo1hi1_a /\ bst r sz2 lo2 hi2 h_bst_rsz2lo2hi2_b,
     [vfun (_: unit) h =>
       let: (x, retv) := vprogs in
       let: (sz1, sz2, v, hi1, r, lo2, l, lo1, hi2, unused) := vghosts in
@@ -89,11 +89,9 @@ exists (1 + sz1 + sz1r2), (sz2r2), (vr22), ((if hi1r2 <= v2 then v2 else hi1r2))
 exists (x :-> v2 \+ x .+ 1 :-> l2 \+ x .+ 2 :-> lr22 \+ h_bst_l2sz1lo1hi1_a \+ h_bst_lr22sz1r2lo1r2hi1r2_513r2);
 exists (h_bst_rr22sz2r2lo2r2hi2r2_514r2);
 sslauto.
-rewrite (addnC 1) ?addnA; auto. (* TODO: convert to Coq's native nat? *)
 unfold_constructor 2;
 exists (sz1), (sz1r2), (v2), (hi1r2), (hi1), (lo1), (lo1r2), (l2), (lr22);
 exists (h_bst_l2sz1lo1hi1_a);
 exists (h_bst_lr22sz1r2lo1r2hi1r2_513r2);
 sslauto.
 Qed.
-
