examples/bst_right_rotate.v
@@ -1,0 +1,97 @@
+From mathcomp
+Require Import ssreflect ssrbool ssrnat eqtype seq ssrfun.
+From fcsl
+Require Import prelude pred pcm unionmap heap.
+From HTT
+Require Import stmod stsep stlog stlogR.
+From SSL
+Require Import core.
+
+Inductive bst (x : ptr) (sz : nat) (lo : nat) (hi : nat) (h : heap) : Prop :=
+| bst_1 of x == null of
+  hi == 0 /\ lo == 7 /\ sz == 0 /\ h = empty
+| bst_2 of (x == null) = false of
+  exists (sz1 : nat) (sz2 : nat) (v : nat) (hi2 : nat) (hi1 : nat) (lo1 : nat) (lo2 : nat) (l : ptr) (r : ptr),
+  exists h_bst_lsz1lo1hi1_513 h_bst_rsz2lo2hi2_514,
+  0 <= sz1 /\ 0 <= sz2 /\ 0 <= v /\ hi == (if hi2 <= v then v else hi2) /\ hi1 <= v /\ lo == (if v <= lo1 then v else lo1) /\ sz == 1 + sz1 + sz2 /\ v <= 7 /\ v <= lo2 /\ h = x :-> v \+ x .+ 1 :-> l \+ x .+ 2 :-> r \+ h_bst_lsz1lo1hi1_513 \+ h_bst_rsz2lo2hi2_514 /\ bst l sz1 lo1 hi1 h_bst_lsz1lo1hi1_513 /\ bst r sz2 lo2 hi2 h_bst_rsz2lo2hi2_514.
+
+Lemma pure1 sz2l2 sz2 sz1l2 : 0 <= sz2l2 -> 0 <= sz2 -> 0 <= 1 + sz1l2 + sz2l2 -> 0 <= sz1l2 -> 0 <= 1 + sz2l2 + sz2. Admitted.
+Hint Resolve pure1: ssl_pure.
+Lemma pure2 sz1l2 sz2l2 sz2 : 0 <= sz2l2 -> 0 <= sz2 -> 0 <= 1 + sz1l2 + sz2l2 -> 0 <= sz1l2 -> sz1l2 + 1 + sz2l2 + sz2 == 1 + sz1l2 + sz2l2 + sz2. Admitted.
+Hint Resolve pure2: ssl_pure.
+Lemma pure3 lo2l2 v2 vl22 hi2l2 lo2 hi1l2 : (if hi2l2 <= vl22 then vl22 else hi2l2) <= v2 -> hi1l2 <= vl22 -> vl22 <= 7 -> 0 <= v2 -> v2 <= lo2 -> 0 <= vl22 -> vl22 <= lo2l2 -> v2 <= 7 -> hi2l2 <= v2. Admitted.
+Hint Resolve pure3: ssl_pure.
+Lemma pure4 lo2l2 v2 vl22 hi2l2 lo2 hi1l2 : (if hi2l2 <= vl22 then vl22 else hi2l2) <= v2 -> hi1l2 <= vl22 -> vl22 <= 7 -> 0 <= v2 -> v2 <= lo2 -> 0 <= vl22 -> vl22 <= lo2l2 -> v2 <= 7 -> vl22 <= (if v2 <= lo2l2 then v2 else lo2l2). Admitted.
+Hint Resolve pure4: ssl_pure.
+
+Definition bst_right_rotate_type :=
+  forall (vprogs : ptr * ptr),
+  {(vghosts : nat * nat * nat * nat * ptr * nat * nat * ptr * nat * ptr)},
+  STsep (
+    fun h =>
+      let: (x, retv) := vprogs in
+      let: (sz1, sz2, v, hi1, l, lo2, lo1, r, hi2, unused) := vghosts in
+      exists h_bst_lsz1lo1hi1_a h_bst_rsz2lo2hi2_b,
+      0 <= sz1 /\ 0 <= sz2 /\ 0 <= v /\ hi1 <= v /\ (l == null) = false /\ v <= 7 /\ v <= lo2 /\ h = retv :-> unused \+ x :-> v \+ x .+ 1 :-> l \+ x .+ 2 :-> r \+ h_bst_lsz1lo1hi1_a \+ h_bst_rsz2lo2hi2_b /\ bst l sz1 lo1 hi1 h_bst_lsz1lo1hi1_a /\ bst r sz2 lo2 hi2 h_bst_rsz2lo2hi2_b,
+    [vfun (_: unit) h =>
+      let: (x, retv) := vprogs in
+      let: (sz1, sz2, v, hi1, l, lo2, lo1, r, hi2, unused) := vghosts in
+      exists sz3 sz4 v3 hi3 lo4 l3 lo3 hi4 y,
+      exists h_bst_l3sz3lo3hi3_515 h_bst_xsz4lo4hi4_516,
+      0 <= sz3 /\ 0 <= sz4 /\ 0 <= v3 /\ hi3 <= v3 /\ sz3 + sz4 == sz1 + sz2 /\ v3 <= 7 /\ v3 <= lo4 /\ h = retv :-> y \+ y :-> v3 \+ y .+ 1 :-> l3 \+ y .+ 2 :-> x \+ h_bst_l3sz3lo3hi3_515 \+ h_bst_xsz4lo4hi4_516 /\ bst l3 sz3 lo3 hi3 h_bst_l3sz3lo3hi3_515 /\ bst x sz4 lo4 hi4 h_bst_xsz4lo4hi4_516
+    ]).
+
+Program Definition bst_right_rotate : bst_right_rotate_type :=
+  Fix (fun (bst_right_rotate : bst_right_rotate_type) vprogs =>
+    let: (x, retv) := vprogs in
+    Do (
+      l2 <-- @read ptr (x .+ 1);
+      if l2 == null
+      then
+        ret tt
+      else
+        rl22 <-- @read ptr (l2 .+ 2);
+        (l2 .+ 2) ::= x;;
+        retv ::= l2;;
+        (x .+ 1) ::= rl22;;
+        ret tt
+    )).
+Obligation Tactic := intro; move=>[x retv]; ssl_program_simpl.
+Next Obligation.
+ssl_ghostelim_pre.
+move=>[[[[[[[[[sz1 sz2] v2] hi1] l2] lo2] lo1] r2] hi2] unused2].
+ex_elim h_bst_l2sz1lo1hi1_a h_bst_r2sz2lo2hi2_b.
+move=>[phi_self0] [phi_self1] [phi_self2] [phi_self3] [phi_self4] [phi_self5] [phi_self6].
+move=>[sigma_self].
+subst.
+move=>[H_bst_l2sz1lo1hi1_a H_bst_r2sz2lo2hi2_b].
+ssl_ghostelim_post.
+ssl_read (x .+ 1).
+ssl_open.
+ssl_open_post H_bst_l2sz1lo1hi1_a.
+ssl_open_post H_bst_l2sz1lo1hi1_a.
+ex_elim sz1l2 sz2l2 vl22 hi2l2 hi1l2.
+ex_elim lo1l2 lo2l2 ll22 rl22.
+ex_elim h_bst_ll22sz1l2lo1l2hi1l2_513l2 h_bst_rl22sz2l2lo2l2hi2l2_514l2.
+move=>[phi_bst_l2sz1lo1hi1_a0] [phi_bst_l2sz1lo1hi1_a1] [phi_bst_l2sz1lo1hi1_a2] [phi_bst_l2sz1lo1hi1_a3] [phi_bst_l2sz1lo1hi1_a4] [phi_bst_l2sz1lo1hi1_a5] [phi_bst_l2sz1lo1hi1_a6] [phi_bst_l2sz1lo1hi1_a7] [phi_bst_l2sz1lo1hi1_a8].
+move=>[sigma_bst_l2sz1lo1hi1_a].
+subst.
+move=>[H_bst_ll22sz1l2lo1l2hi1l2_513l2 H_bst_rl22sz2l2lo2l2hi2l2_514l2].
+ssl_read (l2 .+ 2).
+ssl_write (l2 .+ 2).
+ssl_write_post (l2 .+ 2).
+ssl_write retv.
+ssl_write_post retv.
+ssl_write (x .+ 1).
+ssl_write_post (x .+ 1).
+ssl_emp;
+exists (sz1l2), (1 + sz2l2 + sz2), (vl22), (hi1l2), ((if v2 <= lo2l2 then v2 else lo2l2)), (ll22), (lo1l2), ((if hi2 <= v2 then v2 else hi2)), (l2);
+exists (h_bst_ll22sz1l2lo1l2hi1l2_513l2);
+exists (x :-> v2 \+ x .+ 1 :-> rl22 \+ x .+ 2 :-> r2 \+ h_bst_rl22sz2l2lo2l2hi2l2_514l2 \+ h_bst_r2sz2lo2hi2_b);
+sslauto.
+unfold_constructor 2;
+exists (sz2l2), (sz2), (v2), (hi2), (hi2l2), (lo2l2), (lo2), (rl22), (r2);
+exists (h_bst_rl22sz2l2lo2l2hi2l2_514l2);
+exists (h_bst_r2sz2lo2hi2_b);
+sslauto.
+Qed.
