examples/listmorph.v
@@ -1,0 +1,121 @@
+From mathcomp
+Require Import ssreflect ssrbool ssrnat eqtype seq ssrfun.
+From fcsl
+Require Import prelude pred pcm unionmap heap.
+From HTT
+Require Import stmod stsep stlog stlogR.
+From SSL
+Require Import core.
+
+Inductive lseg (x : ptr) (s : seq nat) (h : heap) : Prop :=
+| lseg_1 of x == null of
+  @perm_eq nat_eqType (s) (nil) /\ h = empty
+| lseg_2 of (x == null) = false of
+  exists (v : nat) (s1 : seq nat) (nxt : ptr),
+  exists h_lseg_nxts1_521,
+  @perm_eq nat_eqType (s) ([:: v] ++ s1) /\ h = x :-> v \+ x .+ 1 :-> nxt \+ h_lseg_nxts1_521 /\ lseg nxt s1 h_lseg_nxts1_521.
+
+Inductive lseg2 (x : ptr) (y : ptr) (s : seq nat) (h : heap) : Prop :=
+| lseg2_1 of x == y of
+  @perm_eq nat_eqType (s) (nil) /\ h = empty
+| lseg2_2 of (x == y) = false of
+  exists (v : nat) (s1 : seq nat) (nxt : ptr),
+  exists h_lseg2_nxtys1_522,
+  @perm_eq nat_eqType (s) ([:: v] ++ s1) /\ h = x :-> v \+ x .+ 1 :-> nxt \+ h_lseg2_nxtys1_522 /\ lseg2 nxt y s1 h_lseg2_nxtys1_522.
+
+Lemma lseg_perm_eq_trans11 x h s_1 s_2 : perm_eq s_1 s_2 -> lseg x s_1 h -> lseg x s_2 h. Admitted.
+Hint Resolve lseg_perm_eq_trans11: ssl_pred.
+Lemma lseg2_perm_eq_trans12 x y h s_1 s_2 : perm_eq s_1 s_2 -> lseg2 x y s_1 h -> lseg2 x y s_2 h. Admitted.
+Hint Resolve lseg2_perm_eq_trans12: ssl_pred.
+Lemma pure13 : @perm_eq nat_eqType (nil) (nil). Admitted.
+Hint Resolve pure13: ssl_pure.
+Lemma pure14 : null == null. Admitted.
+Hint Resolve pure14: ssl_pure.
+Lemma pure15 vx2 s1x : @perm_eq nat_eqType ([:: vx2] ++ s1x) ([:: vx2] ++ s1x). Admitted.
+Hint Resolve pure15: ssl_pure.
+
+Definition listmorph_type :=
+  forall (vprogs : ptr * ptr),
+  {(vghosts : seq nat)},
+  STsep (
+    fun h =>
+      let: (x, r) := vprogs in
+      let: (s) := vghosts in
+      exists h_lseg2_xs_523,
+      h = r :-> null \+ h_lseg2_xs_523 /\ lseg2 x null s h_lseg2_xs_523,
+    [vfun (_: unit) h =>
+      let: (x, r) := vprogs in
+      let: (s) := vghosts in
+      exists y,
+      exists h_lseg_ys_524,
+      h = r :-> y \+ h_lseg_ys_524 /\ lseg y s h_lseg_ys_524
+    ]).
+
+Program Definition listmorph : listmorph_type :=
+  Fix (fun (listmorph : listmorph_type) vprogs =>
+    let: (x, r) := vprogs in
+    Do (
+      if x == null
+      then
+        ret tt
+      else
+        nxtx2 <-- @read ptr (x .+ 1);
+        listmorph (nxtx2, r);;
+        y12 <-- @read ptr r;
+        (x .+ 1) ::= y12;;
+        r ::= x;;
+        ret tt
+    )).
+Obligation Tactic := intro; move=>[x r]; ssl_program_simpl.
+Next Obligation.
+ssl_ghostelim_pre.
+move=>s.
+ex_elim h_lseg2_xs_523.
+move=>[sigma_self].
+subst.
+move=>H_lseg2_xs_523.
+ssl_ghostelim_post.
+ssl_open.
+ssl_open_post H_lseg2_xs_523.
+move=>[phi_lseg2_xs_5230].
+move=>[sigma_lseg2_xs_523].
+subst.
+ssl_emp;
+exists (null);
+exists (empty);
+sslauto.
+unfold_constructor 1;
+sslauto.
+ssl_open_post H_lseg2_xs_523.
+ex_elim vx2 s1x nxtx2.
+ex_elim h_lseg2_nxtx2s1x_522x.
+move=>[phi_lseg2_xs_5230].
+move=>[sigma_lseg2_xs_523].
+subst.
+move=>H_lseg2_nxtx2s1x_522x.
+ssl_read (x .+ 1).
+ssl_call_pre (r :-> null \+ h_lseg2_nxtx2s1x_522x).
+ssl_call (s1x).
+exists (h_lseg2_nxtx2s1x_522x);
+sslauto.
+move=>h_call1.
+ex_elim y12.
+ex_elim h_lseg_y12s1x_5241.
+move=>[sigma_call1].
+subst.
+move=>H_lseg_y12s1x_5241.
+store_valid.
+ssl_read r.
+ssl_write (x .+ 1).
+ssl_write_post (x .+ 1).
+ssl_write r.
+ssl_write_post r.
+ssl_emp;
+exists (x);
+exists (x :-> vx2 \+ x .+ 1 :-> y12 \+ h_lseg_y12s1x_5241);
+sslauto.
+unfold_constructor 2;
+exists (vx2), (s1x), (y12);
+exists (h_lseg_y12s1x_5241);
+sslauto.
+Qed.
